\section{Integration of Complex Functions (Lec. 7)}
Assume \((X, \mathfrak{B}, \mu)\) is a measure space.
\begin{definition}
    A measurable function \(f:X\rightarrow \mathbb{C}\) is called integrable (or $\mu$-integrable) if
    \begin{align*}
        \int\limits_{X}|f|d\mu < \infty.
    \end{align*}
\end{definition}
Denote by \(\mathcal{L}^1(X, \mathfrak{B}, d\mu)\), \(\mathcal{L}^1(X, d\mu)\) or \(\mathcal{L}_{\mathbb{C}}^{1}\) the set of integrable
functions. This is also a vector space over $\mathbb{C}$, since
\begin{align*}
    |f + g| \leq |f| + |g|, \ |cf| = |c||f| \ (c\in \mathbb{C}), \\
    \text{and the other axioms are should be easy}.
\end{align*}
This vector space is spanned by positive functions, since
\begin{align*}
    f = \text{Re}(f)_{+} - \text{Re}(f)_{-} + i\text{Im}(f)_{+} - i\text{Im}(f)_{-},
\end{align*}
where for a function $h$ we let
\begin{align*}
    h_{+} = \max\left\{h,0\right\}, \ h_{-} = -\min\left\{ h,0 \right\},
\end{align*}
and if \(f\in \mathcal{L}^{1}(X, d\mu)\), then
\begin{align*}
    (\text{Re}(f))_{\pm}, (\text{Im}(f))_{\pm} \in \mathcal{L}^{1}(X, d\mu),
\end{align*}
as
\begin{align*}
    |(\text{Re}(f))_{\pm}|, |(\text{Im}(f))_{\pm}| \leq |f|.
\end{align*}

\begin{prop}
    The integral extends uniquely from the positive integrable functions to a linear function (functional?) \(\mathcal{L}^{1}(X, d\mu) \rightarrow \mathbb{C}\),
    that is, to a map s.t.
    \begin{align*}
        \int\limits_{X}(f + g)d\mu = \int\limits_{X}fd\mu + \int\limits_{X}gd\mu, \\
        \int\limits_{X}cfd\mu = c \int\limits_{X}fd\mu, \ c\in\mathbb{C}.
    \end{align*}
\end{prop}
\begin{proof}
    Uniqueness is clear, as positive functions in \(\mathcal{L}^{1}(X, d\mu)\) spans the entire space. We first extend the integral to real
    integrable functions by letting
    \begin{align*}
        \int\limits_{X}(g-h)d\mu \eqdef \int\limits_{X}gd\mu - \int\limits_{X}hd\mu, 
    \end{align*}
    for \(g,h\in \mathcal{L}^{1}(X,d\mu), \ g,h\geq0\).

    This is well-defined, since if
    \begin{align*}
        g - h = g' - h',
    \end{align*}
    then \(g+h' = h + g'\) and hence \(\int\limits_{X}gd\mu + \int\limits_{X}h'd\mu = \int\limits_{X}g'd\mu + \int\limits_{X}h'd\mu\).
    Now we extend the integral to the entire space \(\mathcal{L}'(X,d\mu)\) by
    \begin{align*}
        \int\limits_{X}fd\mu \eqdef \int\limits_{X} (\text{Re}(f))d\mu + i \int\limits_{X}(\text{Im}(f))d\mu.
    \end{align*}
    We easily get that by definition:
    \begin{align*}
        \int\limits_{X}(f_1+f_2)d\mu = \int\limits_{X}f_1d\mu + \int\limits_{X}f_2d\mu, \ \forall f_1, f_2 \in \mathcal{L}^{1}(X, d\mu),
    \end{align*}
    and
    \begin{align*}
        \int\limits_{X}cfd\mu = c\int\limits_{X}fd\mu \ \forall f\in \mathcal{L}^{1}(X,d\mu) \ \forall c\geq 0.
    \end{align*}

    In order to prove the last property for all \(c\in\mathbb{C}\), it remains to check it for \(c=-1\) and \(c=i\).

    For \(c=-1\) it follows, since if \(g,h\geq0\), then
    \begin{eqnarray*}
        \int\limits_{X}\left( -(g-h) \right)d\mu &=& \int\limits_{X}\left( h-g \right)d\mu \\
        &=& \int\limits_{X} h d\mu - \int\limits_{X} gd\mu \\
        &=& - \int\limits_{X}\left( g- h \right)d\mu.
    \end{eqnarray*}
    Similarly, for \(c=i\) it is proved by a simple computation:
    \begin{eqnarray*}
        \int\limits_{X} i fd\mu &=& \int\limits_{X} \text{Re}(if)d\mu + i\int\limits_{X}\text{Im}(if)d\mu \\
        &=& \int\limits_{X}\left( -\text{Im}(f) \right)d\mu + i \int\limits_{X} \left( \text{Re}(f) \right)d\mu \\
        &=& i\left( \int\limits_{X}\left( \text{Re}(f) \right) d\mu + i\int\limits_{X} \left( \text{Im}(f) \right)d\mu\right) \\
        &=& i\int\limits_{X} fd\mu.
    \end{eqnarray*}
\end{proof}
\begin{prop}[Triangle Inequality]
    For every \(f\in \mathcal{L}^{1}(X,d\mu)\) we have
    \begin{align*}
        \Big|\int\limits_{X}fd\mu\Big| \leq \int\limits_{X}|f|d\mu.
    \end{align*}
\end{prop}
\begin{proof}
    Choose \(z\in \Pi\eqdef \left\{ w\in\mathbb{C} : |w|=1 \right\}\) s.t.
    \begin{align*}
        z\int\limits_{X}fd\mu \geq 0.
    \end{align*}
    Then
    \begin{eqnarray*}
        \Big|\int\limits_{X} fd\mu \Big| &=& \Big|z\int\limits_{X}\Big| \\
        &=& z \int\limits_{X}fd\mu \\
        &=& \int\limits_{X}zfd\mu \\
        &=& \int\limits_{X}\text{Re}(zf)d\mu + i \cancel{\int\limits_{X}\text{Im}(zf)d\mu} \\
        &=& \int\limits_{X}\left(\text{Re}(zf)\right)_{+}d\mu - \int\limits_{X}\left(\text{Re}(zf)\right)_{-}d\mu \\
        &\leq& \int\limits_{X}\left(\text{Re}(zf)\right)_{+}d\mu \\
        &\leq& \int\limits_{X}|f|d\mu,
    \end{eqnarray*}
    since \(\left( \text{Re}(zf) \right)_{+} \leq |f|\).
\end{proof}